#   n3 definition of some list functions
#
# $Id: list.n3,v 1.3 2010-03-26 20:41:54 timbl Exp $

@prefix rdf: <http://www.w3.org/1999/02/22-rdf-syntax-ns#> .
@prefix rdfs: <http://www.w3.org/2000/01/rdf-schema#> .
@prefix doc: <http://www.w3.org/2000/01/pim/doc#>.
@prefix log: <http://www.w3.org/2000/10/swap/log#>.
@prefix owl: <http://www.w3.org/2002/07/owl#>.
@prefix vs: <http://www.w3.org/2003/06/sw-vocab-status/ns#> .
@prefix xsd: <http://www.w3.org/2001/XMLSchema#> .

@prefix list: <http://www.w3.org/2000/10/swap/list#>.
@prefix : <#>.

list:append a rdf:Property, owl:FunctionalProperty;
    rdfs:label "append";
    rdfs:domain log:List;
    rdfs:comment """
Iff the subject is a list of lists and the concatenation of all those lists 
is the object, then this is true.
eg  ( (1 2) (3 4) ) list:append (1 2 3 4).
The object can be calculated as a function of the subject.
""";
    rdfs:isDefinedBy <>.

list:first a rdf:Property, owl:FunctionalProperty;
    rdfs:label "first";
    rdfs:domain log:List;
    rdfs:comment """
Iff the subject is a list and the object is the first thing that list, then this is true.
The object can be calculated as a function of the list.
""";
    vs:term_status "unstable";
    rdfs:isDefinedBy <>.

list:in a rdf:Property;
    rdfs:label "in";
    rdfs:range log:List;
    rdfs:comment """
Iff the object is a list and the subject is in that list, then this is true.
""";
    rdfs:isDefinedBy <>.

list:last a rdf:Property, owl:FunctionalProperty;
    rdfs:label "in";
    rdfs:domain log:List;
    rdfs:comment """
Iff the subject is a list and the object is the last thing that list, then this is true.
The object can be calculated as a function of the list.
""";
    rdfs:isDefinedBy <>.

list:length a rdf:Property, owl:FunctionalProperty;
    rdfs:label "length";
    rdfs:domain log:List;
    rdfs:range xsd:integer;
    rdfs:comment """
Iff the subject is a list and the object is the last thing that list, then this is true.
The object can be calculated as a function of the list.
""";
    vs:term_status "unstable";
    rdfs:isDefinedBy <>.

list:member a rdf:Property;
    rdfs:label "member";
    rdfs:domain log:List;
    rdfs:comment """
Iff the subject is a list and the object is in that list, then this is true.
""";
    rdfs:isDefinedBy <>.

list:memberAt a rdf:Property;
    rdfs:label "memberAt";
    rdfs:domain log:List;
    rdfs:comment """
Iff the subject is a list composed of a list and integer position,
and the object exists within that list at the specified position, then this is true.
The object can be calculated as a function of the subject.
The position can be calculated as a function of the first component of the subject and the object.
""";
    vs:term_status "unstable";
    rdfs:isDefinedBy <>.

list:remove a rdf:Property, owl:FunctionalProperty;
    rdfs:label "remove";
    rdfs:domain log:List;
    rdfs:range log:List;
    rdfs:comment """
Iff the subject is a list of two lists and the object is a list composed of the
members of the first component of the subject up to but not including the second component
of the subject, then this is true.
eg ( (1 2 3 4) (3 4) ) list:remove (1 2).
The object can be calculated as a function of the subject.
""";
    vs:term_status "unstable";
    rdfs:isDefinedBy <>.

